theories/sts.v
@@ -9,19 +9,17 @@ Import uPred.
 Definition sts_stateUR := authUR (gmapUR positive (exclR (leibnizC positive))).
 
 Definition sts_relUR :=
-  authUR (gmapUR positive (agreeR (leibnizC (positive → positive → Prop)))).
+  authUR (gmapUR positive (agreeR (leibnizC ((positive → positive → Prop) * (positive → positive → Prop))))).
 
 Definition STS_states : Type := gmap positive positive.
-Definition STS_rels : Type := gmap positive (positive → positive → Prop).
+Definition STS_rels : Type := gmap positive ((positive → positive → Prop) * (positive → positive → Prop)).
 
 (** The CMRA for the thread pool. *)
 Class STSG Σ :=
   { sts_state_inG :> inG Σ sts_stateUR;
-    sts_rel_pub_inG :> inG Σ sts_relUR;
-    sts_rel_priv_inG :> inG Σ sts_relUR;
+    sts_rel_inG :> inG Σ sts_relUR;
     sts_state_name : gname;
-    sts_rel_pub_name : gname;
-    sts_rel_priv_name : gname; }.
+    sts_rel_name : gname; }.
 
 Section definitionsS.
   Context `{STSG Σ} `{Countable A}.
@@ -32,54 +30,56 @@ Section definitionsS.
   Definition convert_rel (R : A → A → Prop) : positive → positive → Prop :=
     λ x y, ∃ a b, x = encode a ∧ y = encode b ∧ R a b.
 
-  Definition sts_rel_pub (i : positive) (R : A → A → Prop) : iProp Σ :=
-    own (A := sts_relUR) sts_rel_pub_name (◯ {[ i := to_agree (convert_rel R) ]}).
+  Definition sts_rel (i : positive) (R : A → A → Prop) (P : A → A → Prop) : iProp Σ :=
+    own (A := sts_relUR) sts_rel_name (◯ {[ i := to_agree ((convert_rel R,convert_rel P)) ]}).
 
-  Definition sts_rel_priv (i : positive) (R : A → A → Prop) : iProp Σ :=
-    own (A := sts_relUR) sts_rel_priv_name (◯ {[ i := to_agree (convert_rel R) ]}).
-
-  Definition sts_subset (fr_pub fr_priv : STS_rels) : Prop :=
-    ∀ i (r_pub r_priv : positive → positive → Prop), fr_pub !! i = Some r_pub → fr_priv !! i = Some r_priv →
-                      (∀ a b, r_pub a b → r_priv a b). 
+  Definition sts_subset (fr : STS_rels) : Prop :=
+    ∀ i (r r' : positive → positive → Prop),
+      fr !! i = Some (r,r') → (∀ a b, r a b → r' a b). 
 
   (* very weird bug!!!
      Any two of these conjuncts are ok on their own but not all three!
      But, it works with program!!!!!!!!!!! *)
-  Program Definition sts_full `{STSG Σ} (fs : STS_states) (fr_pub fr_priv : STS_rels) : iProp Σ
-    := ((⌜dom (gset positive) fs = dom (gset positive) fr_priv⌝ ∧ 
-        ⌜dom (gset positive) fr_priv = dom (gset positive) fr_pub⌝)
-        ∗ ⌜sts_subset fr_pub fr_priv⌝
+  Program Definition sts_full `{STSG Σ} (fs : STS_states) (fr : STS_rels) : iProp Σ
+    := (⌜dom (gset positive) fs = dom (gset positive) fr⌝
+        (* ∗ ⌜sts_subset fr⌝ *)
         ∗ own (A := sts_stateUR) sts_state_name (● (Excl <$> fs))
-        ∗ own (A := sts_relUR) sts_rel_pub_name (● (to_agree <$> fr_pub))
-        ∗ own (A := sts_relUR) sts_rel_priv_name (● (to_agree <$> fr_priv)))%I.
+        ∗ own (A := sts_relUR) sts_rel_name (● (to_agree <$> fr)))%I.
 
-  Definition related_sts (fs gs : STS_states) (fr gr : STS_rels) : Prop :=
+  Definition related_sts_pub (fs gs : STS_states) (fr gr : STS_rels) : Prop :=
     dom (gset positive) fs ⊆ dom (gset positive) gs ∧
     dom (gset positive) fr ⊆ dom (gset positive) gr ∧
-    ∀ i x y r r', fs !! i = Some x → gs !! i = Some y →
-                  fr !! i = Some r → gr !! i = Some r' → r = r' ∧ rtc r x y.
+    (* (∀ i (r r' : positive → positive → Prop), fr !! i = None → gr !! i = Some (r,r') → *)
+    (*                                           (∀ a b, r a b → r' a b)) ∧ *)
+    ∀ i x y r1 r2 r1' r2', fs !! i = Some x → gs !! i = Some y →
+                           fr !! i = Some (r1,r2) → gr !! i = Some (r1',r2') →
+                           r1 = r1' ∧ r2 = r2' ∧ rtc r1 x y.
 
-  Global Instance sts_rel_pub_Persistent i R : Persistent (sts_rel_pub i R).
+  Definition related_sts_priv (fs gs : STS_states) (fr gr : STS_rels) : Prop :=
+    dom (gset positive) fs ⊆ dom (gset positive) gs ∧
+    dom (gset positive) fr ⊆ dom (gset positive) gr ∧
+    (* (∀ i (r r' : positive → positive → Prop), fr !! i = None → gr !! i = Some (r,r') → *)
+    (*                                           (∀ a b, r a b → r' a b)) ∧ *)
+    ∀ i x y r1 r2 r1' r2', fs !! i = Some x → gs !! i = Some y →
+                           fr !! i = Some (r1,r2) → gr !! i = Some (r1',r2') →
+                           r1 = r1' ∧ r2 = r2' ∧ (rtc (λ x y, (r1 x y ∨ r2 x y)) x y).
+    
+
+  Global Instance sts_rel_Persistent i R P : Persistent (sts_rel i R P).
   Proof. apply _. Qed.
 
-  Global Instance sts_rel_priv_Persistent i R : Persistent (sts_rel_priv i R).
-  Proof. apply _. Qed.
-
-  Global Instance sts_rel_pub_Timeless i R : Timeless (sts_rel_pub i R).
-  Proof. apply _. Qed.
-
-  Global Instance sts_rel_priv_Timeless i R : Timeless (sts_rel_priv i R).
+  Global Instance sts_rel_Timeless i R P : Timeless (sts_rel i R P).
   Proof. apply _. Qed.
 
   Global Instance sts_state_Timeless i x : Timeless (sts_state i x).
   Proof. apply _. Qed.
 
-  Global Instance sts_full_Timeless fs fr_pub fr_priv : Timeless (sts_full fs fr_pub fr_priv).
+  Global Instance sts_full_Timeless fs fr : Timeless (sts_full fs fr).
   Proof. apply _. Qed.
 
 End definitionsS.
 
-Typeclasses Opaque sts_state sts_rel_pub sts_rel_priv sts_full related_sts.
+Typeclasses Opaque sts_state sts_rel sts_full related_sts_pub related_sts_priv.
 
 Lemma rtc_implies {A : Type} (R Q : A → A → Prop) (x y : A) :
   (∀ r q, R r q → Q r q) →
@@ -91,8 +91,19 @@ Proof.
   - apply Himpl in H.
     apply rtc_once in H. 
     apply rtc_transitive with y; auto.
+Qed.
+
+Lemma rtc_or_intro {A : Type} (R Q : A → A → Prop) (x y : A) :
+  rtc (λ a b, R a b) x y →
+  rtc (λ a b, R a b ∨ Q a b) x y.
+Proof.
+  intros HR. induction HR.
+  - done.
+  - apply rtc_transitive with y; auto. 
+    apply rtc_once. by left.
 Qed. 
 
+    
 Section STS.
   Context `{STSG Σ} `{Countable A}.
   Implicit Types x y : positive.
@@ -113,103 +124,108 @@ Section STS.
       by apply elem_of_dom in Hin. 
   Qed. 
       
-  Lemma related_sts_refl fs fr : related_sts fs fs fr fr.
+  Lemma related_sts_pub_refl fs fr : related_sts_pub fs fs fr fr.
   Proof.
     split; [|split]; trivial.
     intros; simplify_eq; eauto using rtc_refl.
   Qed.
 
-  Lemma related_sts_trans fs fr gs gr hs hr :
-    related_sts fs gs fr gr → related_sts gs hs gr hr → related_sts fs hs fr hr.
+  Lemma related_sts_priv_refl fs fr : related_sts_priv fs fs fr fr.
+  Proof.
+    split; [|split]; trivial.
+    intros; simplify_eq; eauto using rtc_refl.
+  Qed.
+
+  Lemma related_sts_pub_trans fs fr gs gr hs hr :
+    related_sts_pub fs gs fr gr → related_sts_pub gs hs gr hr →
+    related_sts_pub fs hs fr hr.
   Proof.
     intros [Hf1 [Hf2 Hf3]] [Hg1 [Hg2 Hg3]]; split; [|split]; try by etrans.
-    intros i x y r r' Hfs Hhs Hfr Hhr.
+    intros i x y r1 r2 r1' r2' Hfs Hhs Hfr Hhr.
     specialize (Hf1 i); specialize (Hf2 i);
       revert Hf1 Hf2; rewrite !elem_of_dom; intros Hf1 Hf2.
     destruct Hf1; eauto; destruct Hf2; eauto.
-    edestruct Hf3; eauto; edestruct Hg3; eauto; simplify_eq.
-    split; etrans; eauto.
+    destruct x1. 
+    edestruct Hf3; eauto. edestruct Hg3; eauto; simplify_eq.
+    destruct H6,H4. 
+    split;[auto|split;etrans;eauto]. 
+  Qed.
+  
+  Lemma related_sts_priv_pub_trans fs fr gs gr hs hr :
+    related_sts_priv fs gs fr gr → related_sts_pub gs hs gr hr →
+    related_sts_priv fs hs fr hr.
+  Proof.
+    intros [Hf1 [Hf2 Hf3]] [Hg1 [Hg2 Hg3]]; split; [|split]; try by etrans.
+    intros i x y r1 r2 r1' r2' Hfs Hhs Hfr Hhr.
+    specialize (Hf1 i); specialize (Hf2 i);
+      revert Hf1 Hf2; rewrite !elem_of_dom; intros Hf1 Hf2.
+    destruct Hf1; eauto; destruct Hf2; eauto.
+    destruct x1. 
+    edestruct Hf3; eauto. edestruct Hg3; eauto; simplify_eq.
+    destruct H6,H4. 
+    split;[auto|split;[etrans;eauto|]].
+    subst. etrans; eauto.
+    apply rtc_or_intro. done. 
   Qed.
 
-  Lemma sts_full_rel_priv fs fr_pub fr_priv i R :
-    sts_full fs fr_pub fr_priv -∗ sts_rel_priv i R -∗ ⌜fr_priv !! i = Some (convert_rel R)⌝.
+  Lemma related_sts_pub_priv_trans fs fr gs gr hs hr :
+    related_sts_pub fs gs fr gr → related_sts_priv gs hs gr hr →
+    related_sts_priv fs hs fr hr.
   Proof.
-    rewrite /sts_full /sts_rel_priv.
-    iIntros "[% [_ (_ & _ & H1)]] H2".
-    iDestruct (own_valid_2 with "H1 H2") as %[HR Hv]%auth_valid_discrete;
-      iPureIntro.
-    specialize (Hv i).
-    revert HR; rewrite /= left_id singleton_included;
-      intros [z [Hz HR]]; revert HR; rewrite Some_included_total; intros HR.
-    rewrite lookup_fmap in Hz, Hv.
-    destruct (fr_priv !! i) eqn:Heq; rewrite Heq /= in Hz, Hv; last by inversion Hz.
-    revert Hv; rewrite Hz; intros [u Hu]%to_agree_uninj.
-    revert HR; rewrite -Hu; intros HR%to_agree_included%leibniz_equiv;
-      simplify_eq.
-    inversion Hz as [? ? Hz'|]; simplify_eq.
-    revert Hz'; rewrite -Hu; intros Hz'%to_agree_inj%leibniz_equiv; simplify_eq.
-    by eauto.
+    intros [Hf1 [Hf2 Hf3]] [Hg1 [Hg2 Hg3]]; split; [|split]; try by etrans.
+    intros i x y r1 r2 r1' r2' Hfs Hhs Hfr Hhr.
+    specialize (Hf1 i); specialize (Hf2 i);
+      revert Hf1 Hf2; rewrite !elem_of_dom; intros Hf1 Hf2.
+    destruct Hf1; eauto; destruct Hf2; eauto.
+    destruct x1. 
+    edestruct Hf3; eauto. edestruct Hg3; eauto; simplify_eq.
+    destruct H6,H4. 
+    split;[auto|split;[etrans;eauto|]].
+    subst. etrans; eauto.
+    apply rtc_or_intro. done. 
   Qed.
 
-   Lemma sts_full_rel_pub fs fr_pub fr_priv i R :
-    sts_full fs fr_pub fr_priv -∗ sts_rel_pub i R -∗ ⌜fr_pub !! i = Some (convert_rel R)⌝.
+  Lemma related_sts_priv_trans fs fr gs gr hs hr :
+    related_sts_priv fs gs fr gr → related_sts_priv gs hs gr hr →
+    related_sts_priv fs hs fr hr.
   Proof.
-    rewrite /sts_full /sts_rel_pub.
-    iIntros "[% [_ (_ & H1 & _)]] H2".
-    iDestruct (own_valid_2 with "H1 H2") as %[HR Hv]%auth_valid_discrete;
-      iPureIntro.
-    specialize (Hv i).
-    revert HR; rewrite /= left_id singleton_included;
-      intros [z [Hz HR]]; revert HR; rewrite Some_included_total; intros HR.
-    rewrite lookup_fmap in Hz, Hv.
-    destruct (fr_pub !! i) eqn:Heq; rewrite Heq /= in Hz, Hv; last by inversion Hz.
-    revert Hv; rewrite Hz; intros [u Hu]%to_agree_uninj.
-    revert HR; rewrite -Hu; intros HR%to_agree_included%leibniz_equiv;
-      simplify_eq.
-    inversion Hz as [? ? Hz'|]; simplify_eq.
-    revert Hz'; rewrite -Hu; intros Hz'%to_agree_inj%leibniz_equiv; simplify_eq.
-    by eauto.
-  Qed.
-
-  Lemma sts_full_rel_pub_priv fs fr_pub fr_priv gs gr_pub gr_priv :
-    sts_full fs fr_pub fr_priv -∗
-    ⌜related_sts fs gs fr_pub gr_pub⌝ -∗
-    sts_full gs gr_pub gr_priv -∗
-    ⌜∀ i fi gi, fr_priv !! i = Some fi → gr_priv !! i = Some gi → fi = gi⌝ -∗
-    ⌜related_sts fs gs fr_priv gr_priv⌝.
-  Proof.
-    iIntros "Hffull % Hgfull %". destruct a as (Hfs & Hfrpub & Hrel). 
-    rename a0 into Hpriv. 
-    rewrite /sts_full.
-    iDestruct "Hgfull" as "([% %] & % & _ & _)".
-    iDestruct "Hffull" as "([% %] & % & _ & _)".
-    iPureIntro. 
-    split; auto. split.
-    - by rewrite H2 H5. 
-    - intros i x y r_priv r_priv' Hfsi Hgsi Hfr_privi Hgr_privi.
-      rewrite /sts_subset in H6, H3.
-      assert (is_Some (gr_pub !! i)) as [gr_pub_i Hsomeg].
-      { assert (i ∈ dom (gset positive) gr_priv); [apply elem_of_gmap_dom;eauto|]. 
-        apply elem_of_gmap_dom. by rewrite -H2. }
-      assert (is_Some (fr_pub !! i)) as [fr_pub_i Hsomef].
-      { assert (i ∈ dom (gset positive) fr_priv); [apply elem_of_gmap_dom;eauto|]. 
-        apply elem_of_gmap_dom. by rewrite -H5. }
-      (* specialize H3 with i gr_pub_i r_priv' x y. *)
-      (* specialize H6 with i gr_pub_i r_priv x y. *)
-      assert (fr_pub_i = gr_pub_i ∧ rtc fr_pub_i x y) as [Hfrgrpub Hxy];
-        [apply Hrel with i; auto|].
-      assert (r_priv = r_priv');
-        [apply Hpriv with i; auto|].
-      split; auto.
-      apply rtc_implies with gr_pub_i; try congruence.
-        apply H3 with i; try congruence.  
+    intros [Hf1 [Hf2 Hf3]] [Hg1 [Hg2 Hg3]]; split; [|split]; try by etrans.
+    intros i x y r1 r2 r1' r2' Hfs Hhs Hfr Hhr.
+    specialize (Hf1 i); specialize (Hf2 i);
+      revert Hf1 Hf2; rewrite !elem_of_dom; intros Hf1 Hf2.
+    destruct Hf1; eauto; destruct Hf2; eauto.
+    destruct x1. 
+    edestruct Hf3; eauto. edestruct Hg3; eauto; simplify_eq.
+    destruct H6,H4. 
+    split;[auto|split;[etrans;eauto|]].
+    subst. etrans; eauto.
   Qed. 
+
+  Lemma sts_full_rel fs fr i R P :
+    sts_full fs fr -∗ sts_rel i R P -∗ ⌜fr !! i = Some (convert_rel R,convert_rel P)⌝.
+  Proof.
+    rewrite /sts_full /sts_rel.
+    iIntros "[% [_ H1]] H2".
+    iDestruct (own_valid_2 with "H1 H2") as %[HR Hv]%auth_valid_discrete;
+      iPureIntro.
+    specialize (Hv i).
+    revert HR; rewrite /= left_id singleton_included;
+      intros [z [Hz HR]]; revert HR; rewrite Some_included_total; intros HR.
+    rewrite lookup_fmap in Hz, Hv.
+    destruct (fr !! i) eqn:Heq; rewrite Heq /= in Hz, Hv; last by inversion Hz.
+    revert Hv; rewrite Hz; intros [u Hu]%to_agree_uninj.
+    revert HR; rewrite -Hu; intros HR%to_agree_included%leibniz_equiv;
+      simplify_eq.
+    inversion Hz as [? ? Hz'|]; simplify_eq.
+    revert Hz'; rewrite -Hu; intros Hz'%to_agree_inj%leibniz_equiv; simplify_eq.
+    by eauto.
+  Qed.
       
-  Lemma sts_full_state fs fr_pub fr_priv i a :
-    sts_full fs fr_pub fr_priv -∗ sts_state i a -∗ ⌜fs !! i = Some (encode a)⌝.
+  Lemma sts_full_state fs fr i a :
+    sts_full fs fr -∗ sts_state i a -∗ ⌜fs !! i = Some (encode a)⌝.
   Proof.
     rewrite /sts_full /sts_state.
-    iIntros "[% [_ [H1 _]]] H2".
+    iIntros "[% [H1 _]] H2".
     iDestruct (own_valid_2 with "H1 H2") as %[HR Hv]%auth_valid_discrete;
       iPureIntro.
     specialize (Hv i).
@@ -222,19 +238,15 @@ Section STS.
     apply leibniz_equiv in HR; simplify_eq; eauto.
   Qed.
 
-  Lemma sts_alloc fs fr_pub fr_priv a R Q :
-    (∀ x y, (convert_rel R) x y → (convert_rel Q) x y) →
-    sts_full fs fr_pub fr_priv ==∗
-             ∃ i, sts_full (<[i := encode a ]>fs) (<[i := convert_rel R ]>fr_pub)
-                           (<[i := convert_rel Q ]>fr_priv)
-                           ∗ ⌜i ∉ dom (gset positive) fs⌝
-                           ∗ ⌜i ∉ dom (gset positive) fr_pub⌝
-                           ∗ ⌜i ∉ dom (gset positive) fr_priv⌝
-                  ∗ sts_state i a ∗ sts_rel_pub i R ∗ sts_rel_priv i Q.
+  Lemma sts_alloc fs fr a R P:
+    sts_full fs fr ==∗
+             ∃ i, sts_full (<[i := encode a ]>fs) (<[i := (convert_rel R,convert_rel P) ]>fr)
+                  ∗ ⌜i ∉ dom (gset positive) fs⌝ ∗ ⌜i ∉ dom (gset positive) fr⌝
+                  ∗ sts_state i a ∗ sts_rel i R P.
   Proof.
-    rewrite /sts_full /sts_rel_pub /sts_rel_priv /sts_state.
-    iIntros (HRQ) "[Hd [% [H1 [H2 H2']]]]".
-    iDestruct "Hd" as %[Hd Hd'].
+    rewrite /sts_full /sts_rel /sts_state.
+    iIntros "[Hd [H1 H2]]".
+    iDestruct "Hd" as %Hd.
     iMod (own_update
             (A := sts_stateUR)
             _ _
@@ -252,58 +264,36 @@ Section STS.
             (A := sts_relUR)
             _ _
             (● (to_agree <$>
-                <[fresh (dom (gset positive) fs) := convert_rel R]> fr_pub)
-            ⋅ ◯ {[fresh (dom (gset positive) fs) := to_agree (convert_rel R)]})
+                <[fresh (dom (gset positive) fs) := (convert_rel R,convert_rel P)]> fr)
+            ⋅ ◯ {[fresh (dom (gset positive) fs) := to_agree (convert_rel R,convert_rel P)]})
             with "H2") as "[H2 Hr]".
     { apply auth_update_alloc.
       rewrite fmap_insert /=.
       apply: alloc_singleton_local_update; last done.
       apply (not_elem_of_dom (D := gset positive)).
-      rewrite dom_fmap Hd Hd'.
-      apply is_fresh. }
-    iMod (own_update
-            (A := sts_relUR)
-            _ _
-            (● (to_agree <$>
-                <[fresh (dom (gset positive) fs) := convert_rel Q]> fr_priv)
-            ⋅ ◯ {[fresh (dom (gset positive) fs) := to_agree (convert_rel Q)]})
-            with "H2'") as "[H2' Hr']".
-    { apply auth_update_alloc.
-      rewrite fmap_insert /=.
-      apply: alloc_singleton_local_update; last done.
-      apply (not_elem_of_dom (D := gset positive)).
-      rewrite dom_fmap Hd Hd'.
+      rewrite dom_fmap Hd.
       apply is_fresh. }
     iModIntro.
     iExists _; iFrame.
-    repeat iSplit; try iPureIntro;
-      rewrite ?dom_insert_L ?Hd Hd'; try apply is_fresh; auto.
-    rewrite /sts_subset.
-    intros i r_pub r_priv Hpub Hpriv a' b' Ha'.
-    destruct (decide (fresh (dom (gset positive) fr_pub) = i)).
-    - rewrite e lookup_insert in Hpub, Hpriv. rewrite lookup_insert in Hpriv.
-      inversion Hpub; inversion Hpriv.
-      apply HRQ. congruence.
-    - rewrite lookup_insert_ne in Hpub; auto.
-      rewrite lookup_insert_ne in Hpriv; auto.
-      rewrite /sts_subset in H1. apply H1 with i r_pub; auto. 
+    repeat iSplit; iPureIntro;
+      rewrite ?dom_insert_L ?Hd; by try apply is_fresh.
   Qed.
 
-  Lemma sts_update fs fr_pub fr_priv i a b :
-    sts_full fs fr_pub fr_priv -∗ sts_state i a ==∗
-    sts_full (<[i := encode b ]>fs) fr_pub fr_priv ∗ sts_state i b.
+  Lemma sts_update fs fr i a b :
+    sts_full fs fr -∗ sts_state i a ==∗
+    sts_full (<[i := encode b ]>fs) fr ∗ sts_state i b.
   Proof.
     iIntros "Hsf Hi".
     iDestruct (sts_full_state with "Hsf Hi") as %Hfs.
-    rewrite /sts_full /sts_rel_pub /sts_rel_priv /sts_state.
-    iDestruct "Hsf" as "[Hd [H1 [H2 [H3 H4]]]]".
+    rewrite /sts_full /sts_rel /sts_state.
+    iDestruct "Hsf" as "[Hd [H1 H2]]".
     iDestruct "Hd" as %Hd.
-    iCombine "H2" "Hi" as "H2".
+    iCombine "H1" "Hi" as "H1".
     iMod (own_update (A := sts_stateUR)
             _ _
             (● (<[i := Excl (encode b)]> (Excl <$> fs))
                ⋅ ◯ {[i := Excl (encode b)]})
-            with "H2") as "[H2 Hs]".
+            with "H1") as "[H1 Hs]".
     { apply auth_update.
       apply: singleton_local_update; eauto.
       rewrite lookup_fmap Hfs //=.
